third_party/move/lean/Tests/Move/Modules/Math.lean
@@ -12,8 +12,7 @@ open scoped Move Move.Compiler Move.Spec
 
 move_module Math where
 
-  @[move_public]
-  fun identity {T : Type} (value : T) : T := value
+  public fun identity {T : Type} (value : T) : T := value
 
   spec identity {T : Type} [Inhabited T] (value : T) where
     ensures result = value
